\documentclass[a4paper]{article}

\usepackage[utf8]{inputenc}
\usepackage{microtype}
\usepackage{enumitem}
\usepackage{comment}
\usepackage{float, graphicx}
\usepackage{mathtools, amssymb, mathrsfs}
\usepackage{caption}
\usepackage{subcaption}

\setlength{\parindent}{0em}


\title{3}
\date{}

\begin{document}
\maketitle




Let us assume that we have 2 discrete signals $f(x,y)$ and $g(x,y)$. The size of both is $W_1 \times W_2$. If the sizes of both signals are not the same, we can employ zero-padding to make them of the same size.

The 2D discrete convolution is defined as:
\[f \ast g(u,v) = \sum_{x = 0}^{W_1 -1} \sum_{y = 0}^{W_2 - 1}f(x,y)g(u-x,v-y)\]

The 2D Fourier Transform of a discrete signal is given by:
\[\mathscr{F}(f)(u,v) = \sum_{x = 0}^{W_1 -1} \sum_{y = 0}^{W_2 - 1}f(x,y)e^{-2 \pi j(\frac{ux}{W_1} + \frac{vy}{W_2})}\]

Hence,
\[\mathscr{F}(f\ast g)(u,v) = \sum_{x = 0}^{W_1 -1} \sum_{y = 0}^{W_2 - 1}\sum_{x' = 0}^{W_1 -1} \sum_{y' = 0}^{W_2 - 1}f(x',y')g(x-x',y-y')e^{-2 \pi j(\frac{ux}{W_1} + \frac{vy}{W_2})}\]

We can rearrange the summations to obtain the following:
\[\mathscr{F}(f\ast g)(u,v) = \sum_{x' = 0}^{W_1 -1} \sum_{y' = 0}^{W_2 - 1}f(x',y')\sum_{x = 0}^{W_1 -1} \sum_{y = 0}^{W_2 - 1}g(x-x',y-y')e^{-2 \pi j(\frac{ux}{W_1} + \frac{vy}{W_2})}\]

We note that,
\[\sum_{x = 0}^{W_1 -1} \sum_{y = 0}^{W_2 - 1}g(x-x',y-y')e^{-2 \pi j(\frac{ux}{W_1} + \frac{vy}{W_2})} = \mathscr{F}(g(m-x',n-y'))(u,v)\] 
Also, using the translation property of Fourier transform, we can write:
\[\mathscr{F}(g(m-x',n-y'))(u,v) = \mathscr{F}(g)(u,v)e^{-2 \pi j(\frac{ux'}{W_1} + \frac{vy'}{W_2})} \] 

Hence we can rewrite the original equation as:
\[\mathscr{F}(f\ast g)(u,v) = \sum_{x' = 0}^{W_1 -1} \sum_{y' = 0}^{W_2 - 1}f(x',y') \mathscr{F}(g)(u,v)e^{-2 \pi j(\frac{ux'}{W_1} + \frac{vy'}{W_2})}\]

Rearranging:
\[\mathscr{F}(f\ast g)(u,v) =  \mathscr{F}(g)(u,v)\sum_{x' = 0}^{W_1 -1} \sum_{y' = 0}^{W_2 - 1}f(x',y')e^{-2 \pi j(\frac{ux'}{W_1} + \frac{vy'}{W_2})}\]

Also,

\[\sum_{x' = 0}^{W_1 -1} \sum_{y' = 0}^{W_2 - 1}f(x',y')e^{-2 \pi j(\frac{ux'}{W_1} + \frac{vy'}{W_2})} = \mathscr{F}(f)(u,v)\]

Hence,
\[\mathscr{F}(f\ast g)(u,v) =  \mathscr{F}(g)(u,v)\mathscr{F}(f)(u,v)\]

which is the convolution theorem for 2D Discrete Fourier transforms.

\end{document}

